\documentclass{report}

\include{preamble}
\include{macros}
\include{letterfonts}

\usepackage[Glenn]{fncychap}

\title{\Huge{Lösningar HW 13}}
\author{\huge{}}
\date{}


\begin{document}

\maketitle
\newpage
\pagebreak

\qs{}
{
\textbf{Induktion 1}: Bevisa följande:
\begin{equation}
\sum_{i=1}^{n} i^2 = \frac{n(n+1)(2n+1)}{6}
\end{equation}

\begin{equation}
\sum_{j=1}^{n} (2j-1) = n^2
\end{equation}
}
\sol (1)\\
\textbf{Basfall} $ n = 1$:
\begin{equation*}
\text{V.L:}\:\sum_{i=1}^{1} i^2 = 1;\:\:\:\text{H.L:}\: \frac{1(2)(3)}{6} = 1\:\:\:\:\text{(OK!)}
\end{equation*}
\textbf{Induktionsantagande}:
\begin{equation*}
\sum_{i=1}^{n} i^2 = \frac{n(n+1)(2n+1)}{6}
\end{equation*}
\textbf{Induktionssteget}:
\begin{equation*}
P_{V.L}(n+1) \implies \sum_{i=1}^{n+1} i^2 \iff \sum_{i=1}^{n} i^2 + (n+1)^2 \iff P_{V.L}(n) + (n+1)^2
\end{equation*}
Enligt induktionsantagandet kan vi skriva om $P_{V.L}(n)$ till $\frac{n(n+1)(2n+1)}{6}$, s.a.:
\begin{equation*}
P_{V.L}(n) + (n+1)^2 \iff \frac{n(n+1)(2n+1)}{6} + (n+1)^2	
\end{equation*}
\begin{equation*}
P_{H.L}(n+1) \implies \frac{(n+1)(n+2)(2n+3)}{6} \iff \frac{(n+1)(2n^2+7n+6)}{6} \iff \frac{(n+1)(2n^2+n+6(n+1))}{6}
\end{equation*}
\begin{equation*}
P_{H.L}(n+1) \implies \frac{(n+1)(2n^2+n+6(n+1))}{6} \iff \frac{n(n+1)(2n+1)+6(n+1)^2}{6} \iff \frac{n(n+1)(2n+1)}{6} + (n+1)^2
\end{equation*}
Det sista raden implicerar att $P_{H.L}(n+1) = P_{V.L}(n+1)$. Alltså \textbf{V.S.B}!\\\\

\sol (2)\\
\textbf{Basfall} $n=1$:
\begin{equation*}
\text{V.L:}\:\sum_{i=j}^{1} (2j-1) = 1;\:\:\:\text{H.L:}\: 1^2 = 1\:\:\:\:\text{(OK!)}
\end{equation*}
\textbf{Induktionsantagande}:
\begin{equation*}
\sum_{j=1}^{n} (2j-1)= n^2
\end{equation*}
\textbf{Induktionssteget}:
\begin{equation*}
P_{V.L}(n+1) \implies \sum_{j=1}^{n+1}(2j-1) \iff \sum_{j=1}^{n}(2j-1) + 2(n+1)-1 \iff P_{V.L}(n) + 2n+1
\end{equation*}
Enligt induktionsantagandet kan vi skriva om $P_{V.L}(n)$ till $n^2$, s.a.:
\begin{equation*}
P_{V.L}(n) + 2n+1 \iff n^2 + 2n + 1 \iff (n+1)^2 = P_{V.L}(n+1)
\end{equation*}
\begin{equation*}
P_{H.L}(n+1) \implies (n+1)^2
\end{equation*}
Alltså $P_{H.L}(n+1) = P_{V.L}(n+1)$ \textbf{V.S.B}!
\end{document}
